wip, propagating send_across through kernel descriptions

src/lib/kuiper/Kuiper.SHMem.fst
@@ -3,7 +3,10 @@ module Kuiper.SHMem
 #lang-pulse
 
 open Pulse.Lib.Core
+open Pulse.Lib.SendSync
+open Kuiper.Base
 open Kuiper.Array
+open FStar.Tactics.V2
 module SZ = Kuiper.SizeT
 module T = FStar.Tactics
 
@@ -17,10 +20,23 @@ type shmem_desc =
     len    : SZ.t ->
     shmem_desc
 
+let is_block_array #ty #len (g:gpu_array ty len) 
+  = visibility_of g == block_of
+
+instance is_send_across_block_array
+  (#et:Type0) (#sz:_) 
+  (a:gpu_array et sz { is_block_array a })
+  (#i #j #f #s:_)
+: is_send_across block_of (gpu_pts_to_slice a #f i j s)
+= let i : is_send_across (visibility_of a) (gpu_pts_to_slice a #f i j s)
+   = FStar.Tactics.Typeclasses.solve in
+  i
+
 inline_for_extraction unfold
 let c_shmem (d : shmem_desc) : Type0 =
   match d with
-  | SHArray ty len -> gpu_array ty len
+  | SHArray ty len -> gpu_array ty len 
+   //would be nice to just add as is_block_array refinement here, but it messes with typeclass resolution
 
 inline_for_extraction
 let rec c_shmems (d : list shmem_desc) : Type0 =
@@ -29,9 +45,60 @@ let rec c_shmems (d : list shmem_desc) : Type0 =
   | d :: ds ->
     c_shmem d & c_shmems ds
 
+let c_shmem_inv (#d : shmem_desc) (c:c_shmem d) : prop =
+  match d with
+  | SHArray ty len -> is_block_array #ty #len c 
+
+let rec c_shmems_inv (#ds : list shmem_desc) (c:c_shmems ds) : prop =
+  match ds with
+  | [] -> True
+  | d :: ds -> 
+    let c : c_shmem d & c_shmems ds = c in (* coerce *)
+    c_shmem_inv #d (fst c) /\
+    c_shmems_inv #ds (snd c)
+
+
+// inline_for_extraction
+// let first_ty (d:list shmem_desc { not (Nil? d) }) : Type0 =
+//   match d with
+//   | SHArray ty len::_ -> ty
+
+// instance first_ty_sized (d:list shmem_desc) (_:squash(not (Nil? d))) 
+// : Kuiper.Sized.sized (first_ty d)
+// = match d with
+//   | SHArray ty #sized len::_ -> sized
+
+// inline_for_extraction
+// let first_len (d:list shmem_desc { not (Nil? d) }) : SZ.t =
+//   match d with
+//   | SHArray ty len::_ -> len
+
+// let first (#d:list shmem_desc { not (Nil? d) }) (c:c_shmems d)
+// : gpu_array (first_ty d) (first_len d)
+//  = match d with
+//   | d::ds -> 
+//     let c : c_shmem d & c_shmems ds = c in
+//     fst c
+
 let live_c_shmem #d (c : c_shmem d) : slprop =
   match d with
-  | SHArray ty len -> exists* v. gpu_pts_to_array #ty #len c #1.0R v
+  | SHArray ty len -> 
+    exists* v. gpu_pts_to_array #ty #len c #1.0R v
+
+instance is_send_across_live_c_shmem #d (c:c_shmem d) (_:squash (c_shmem_inv c))
+: is_send_across block_of (live_c_shmem #d c)
+= match d with
+  | SHArray ty len ->
+    let ff (v:_) : is_send_across block_of  (gpu_pts_to_array #ty #len c #1.0R v) =
+      FStar.Tactics.Typeclasses.solve
+    in
+    let ff : is_send_across block_of (exists* v. gpu_pts_to_array #ty #len c #1.0R v) =
+      is_send_across_exists _ #ff
+    in 
+    let ff : is_send_across block_of (live_c_shmem #(SHArray ty len) c)
+      = ff
+    in
+    ff
 
 let rec live_c_shmems #ds (c : c_shmems ds) : slprop =
   match ds with
@@ -39,3 +106,22 @@ let rec live_c_shmems #ds (c : c_shmems ds) : slprop =
   | d :: ds ->
     let c : c_shmem d & c_shmems ds = c in (* coerce *)
     live_c_shmem #d (fst c) ** live_c_shmems #ds (snd c)
+
+let rec is_send_across_live_c_shmems_ #ds (c:c_shmems ds) (pf:squash (c_shmems_inv c))
+: is_send_across block_of (live_c_shmems #ds c)
+= let open FStar.Tactics.Typeclasses in
+  match ds with
+  | [] -> solve #(is_send_across block_of emp)
+  | d::ds ->
+    let c : c_shmem d & c_shmems ds = c in (* coerce *)
+    let s = is_send_across_live_c_shmems_ #ds (snd c) () in
+    let f : is_send_across block_of (live_c_shmem #d (fst c)) = solve in
+    is_send_across_star _ _ #f #s
+
+instance is_send_across_live_c_shmems #ds (c:c_shmems ds) (pf:squash (c_shmems_inv c))
+: is_send_across block_of (live_c_shmems #ds c)
+= is_send_across_live_c_shmems_ #ds c pf
+
+(* 1xn, shared memory *)
+
+
