src/lib/poly/Kuiper.Poly.HReduce.fst
@@ -413,11 +413,12 @@ fn block_teardown
     gpu_pts_to_slice_sum a 0 (v lena) va vr);
 }
 
+
 inline_for_extraction noextract
 let kernel
   (#et:Type0) {| scalar et, real_like et |}
   (lena : szp { lena < max_threads })
-  (a : gpu_array et lena)
+  (a : gpu_array et lena { is_global_array a })
   (#va : erased (seq et))
   (#vr : erased (seq real) { va %~ vr })
   (#_ : squash (Seq.length va == SZ.v lena))
@@ -433,6 +434,10 @@ let kernel
   kpost = kpost lena a va vr;
   kpre =  kpre lena a va vr;
   frame = emp;
+  kpre_sendable=solve;
+  kpost_sendable=solve;
+  full_post_sendable=solve;
+  full_pre_sendable=solve
 }
 
 inline_for_extraction noextract
