src/lib/poly/gemm/Kuiper.Poly.GEMM.Naive2.fst
@@ -182,11 +182,11 @@ let kdesc
   (#lB : mlayout shared cols)
   (#lC : mlayout rows cols)
   {| clayout lA, clayout lB, clayout lC |}
-  (gA : M.gpu_matrix et lA)
+  (gA : M.gpu_matrix et lA { M.is_global_matrix gA })
   (#fA : perm)
-  (gB : M.gpu_matrix et lB)
+  (gB : M.gpu_matrix et lB { M.is_global_matrix gB })
   (#fB : perm)
-  (gC : M.gpu_matrix et lC)
+  (gC : M.gpu_matrix et lC { M.is_global_matrix gC })
   (#eA : ematrix et rows shared)
   (#eB : ematrix et shared cols)
   (#eC : ematrix et rows cols)
@@ -207,6 +207,8 @@ let kdesc
   kpost = kpost comb gA gB gC eA eB eC fA fB;
 
   f = kf comb gA gB gC #eA #eB #eC #fA #fB;
+  kpre_sendable=solve;
+  kpost_sendable=solve;
 }
 
 // FIXME: extraction of this function (in the inst module) is very slow, around
@@ -241,5 +243,5 @@ fn mmcomb_gpu
   ensures
     on gpu_loc (gC |-> MS.mmcomb comb eC eA eB)
 {
-  launch_sync (kdesc comb gA #fA gB #fB gC #eA #eB #eC #());
+  launch_sync (kdesc comb gA gB gC);
 }
